more Compiler.v

Compiler.v
@@ -1,4 +1,3 @@
-
 Require Import Com.
 Require Import Big_Step.
 Require Import Star.
@@ -46,8 +45,8 @@ Lemma lem_exec1I :
                        exec1 P (i,s,stk) c'.
 Proof.
   Reconstr.hobvious Reconstr.Empty
-		    (@Coq.ZArith.BinInt.Z.lt_nge)
-		    (@Coq.ZArith.BinInt.Z.ge, @znth, @exec1, @Coq.ZArith.BinInt.Z.lt).
+                    (@Coq.ZArith.BinInt.Z.lt_nge)
+                    (@Coq.ZArith.BinInt.Z.ge, @znth, @exec1, @Coq.ZArith.BinInt.Z.lt).
 Qed.
 
 (* Helper instruction list functions *)
@@ -57,12 +56,34 @@ Lemma lem_n_succ_znth :
 Proof.
   induction n; sauto.
   - Reconstr.htrivial Reconstr.AllHyps
-		      (@Coq.PArith.Pnat.Pos2Nat.inj_succ, @Coq.PArith.BinPos.Pos.add_1_r)
-		      Reconstr.Empty.
+                      (@Coq.PArith.Pnat.Pos2Nat.inj_succ, @Coq.PArith.BinPos.Pos.add_1_r)
+                      Reconstr.Empty.
   - Reconstr.htrivial Reconstr.AllHyps
-		      (@Coq.PArith.BinPos.Pos.add_1_r, @Coq.PArith.Pnat.Pos2Nat.inj_succ,
+                      (@Coq.PArith.BinPos.Pos.add_1_r, @Coq.PArith.Pnat.Pos2Nat.inj_succ,
                        @Coq.ZArith.Znat.Z2Nat.inj_pos, @Coq.Init.Peano.eq_add_S)
-		      (@znth).
+                      (@znth).
+Qed.
+
+Lemma lem_znth_app :
+  forall xs ys i x, i >= 0 -> znth (size xs + i) (xs ++ ys) x = znth i ys x.
+Proof.
+  assert (forall n (xs ys : list instr) i x, i >= 0 -> n = length xs ->
+                                             znth (Z.of_nat n + i) (xs ++ ys) x = znth i ys x);
+    [idtac | scrush].
+  induction n.
+  - scrush.
+  - assert (HH: Z.of_nat (S n) = Z.of_nat n + 1) by
+        Reconstr.htrivial Reconstr.Empty
+                          (@Coq.ZArith.Znat.Nat2Z.inj_succ)
+                          (@Coq.ZArith.BinIntDef.Z.succ).
+    rewrite HH; clear HH.
+    intros xs ys i x H1 H2.
+    assert (0 <= Z.of_nat n + i) by omega.
+    assert (HH: Z.of_nat n + 1 + i = (Z.of_nat n + i) + 1) by omega.
+    rewrite HH; clear HH.
+    destruct xs; [ scrush | simpl ].
+    rewrite lem_n_succ_znth by scrush.
+    scrush.
 Qed.
 
 Lemma lem_size_succ :
@@ -72,9 +93,9 @@ Proof.
   induction n; sauto.
   - scrush.
   - Reconstr.htrivial Reconstr.AllHyps
-		      (@Coq.PArith.BinPos.Pplus_one_succ_r, @Coq.ZArith.Znat.Zpos_P_of_succ_nat,
+                      (@Coq.PArith.BinPos.Pplus_one_succ_r, @Coq.ZArith.Znat.Zpos_P_of_succ_nat,
                        @Coq.ZArith.BinInt.Pos2Z.inj_succ)
-		      (@Coq.ZArith.BinIntDef.Z.succ, @size).
+                      (@Coq.ZArith.BinIntDef.Z.succ, @size).
   - scrush.
 Qed.
 
@@ -86,16 +107,16 @@ Proof.
   induction xs.
   - sauto.
     + Reconstr.hcrush Reconstr.AllHyps
-		  (@Coq.ZArith.BinInt.Z.ltb_ge)
-		  Reconstr.Empty.
+                  (@Coq.ZArith.BinInt.Z.ltb_ge)
+                  Reconstr.Empty.
     + scrush.
     + scrush.
   - intros.
     assert (HH: i = 0 \/ exists i', i = i' + 1 /\ 0 <= i') by
         Reconstr.hcrush Reconstr.AllHyps
-		        (@Coq.ZArith.BinInt.Z.lt_le_pred, @Coq.ZArith.BinInt.Z.lt_eq_cases,
+                        (@Coq.ZArith.BinInt.Z.lt_le_pred, @Coq.ZArith.BinInt.Z.lt_eq_cases,
                          @Coq.ZArith.BinInt.Z.succ_pred)
-		        (@Coq.ZArith.BinIntDef.Z.succ).
+                        (@Coq.ZArith.BinIntDef.Z.succ).
     destruct HH as [ ? | HH ].
     scrush.
     destruct HH as [ i' HH ].
@@ -106,15 +127,15 @@ Proof.
     sauto.
     + assert ((i' <? size xs) = true).
       Reconstr.hcrush Reconstr.AllHyps
-		      (@Coq.ZArith.BinInt.Z.le_gt_cases, @Coq.Bool.Bool.diff_true_false,
+                      (@Coq.ZArith.BinInt.Z.le_gt_cases, @Coq.Bool.Bool.diff_true_false,
                        @Coq.ZArith.BinInt.Z.ltb_ge, @Coq.ZArith.Zbool.Zlt_is_lt_bool,
                        @Coq.ZArith.BinInt.Z.add_le_mono_r)
-		      (@size).
+                      (@size).
       scrush.
     + assert ((i' <? size xs) = false).
       Reconstr.heasy Reconstr.AllHyps
-		     (@Coq.ZArith.BinInt.Z.ltb_nlt, @Coq.ZArith.BinInt.Z.add_lt_mono_r)
-		     (@size).
+                     (@Coq.ZArith.BinInt.Z.ltb_nlt, @Coq.ZArith.BinInt.Z.add_lt_mono_r)
+                     (@size).
       assert (i' + 1 - (size xs + 1) = i' - size xs) by auto with zarith.
       scrush.
 Qed.
@@ -122,20 +143,20 @@ Qed.
 Lemma lem_size_app : forall xs ys, size (xs ++ ys) = size xs + size ys.
 Proof.
   Reconstr.htrivial Reconstr.Empty
-		    (@Coq.ZArith.Znat.Nat2Z.inj_add, @Coq.Lists.List.app_length)
-		    (@size).
+                    (@Coq.ZArith.Znat.Nat2Z.inj_add, @Coq.Lists.List.app_length)
+                    (@size).
 Qed.
 
 Lemma lem_size_app_le : forall xs ys, size xs <= size (xs ++ ys).
 Proof.
   Reconstr.hobvious Reconstr.Empty
-		    (@Coq.Arith.Plus.le_plus_l, @Coq.ZArith.Znat.Nat2Z.inj_le, @Coq.Lists.List.app_length)
-		    (@size).
+                    (@Coq.Arith.Plus.le_plus_l, @Coq.ZArith.Znat.Nat2Z.inj_le, @Coq.Lists.List.app_length)
+                    (@size).
 Qed.
 
 (* Verification infrastructure *)
 
-Lemma lem_iexec_shift : 
+Lemma lem_iexec_shift :
   forall x n i i' s s' stk stk',
     (n+i',s',stk') = iexec x (n+i,s,stk) <->
     (i',s',stk') = iexec x (i,s,stk).
@@ -156,7 +177,7 @@ Proof.
   induction n.
   - scrush.
   - Reconstr.hcrush Reconstr.Empty
-		    (@lem_size_succ, @lem_nth_append, @Coq.ZArith.Zbool.Zlt_is_lt_bool)
+                    (@lem_size_succ, @lem_nth_append, @Coq.ZArith.Zbool.Zlt_is_lt_bool)
                     Reconstr.Empty.
   - scrush.
 Qed.
@@ -172,9 +193,9 @@ Proof.
   rewrite <- lem_exec1_hlp1 by auto with zarith.
   assert (i < size (P ++ P')) by
       Reconstr.heasy Reconstr.AllHyps
-		     (@lem_size_app_le, @Coq.ZArith.BinInt.Z.le_lt_trans,
+                     (@lem_size_app_le, @Coq.ZArith.BinInt.Z.le_lt_trans,
                       @Coq.ZArith.BinInt.Z.nle_gt, @Coq.ZArith.BinInt.Z.lt_ge_cases)
-		     (@size).
+                     (@size).
   scrush.
 Qed.
 
@@ -185,28 +206,6 @@ Proof.
   induction H.
   - scrush.
   - pose @star_step; pose lem_exec1_appendR; scrush.
-Qed.
-
-Lemma lem_znth_app :
-  forall xs ys i x, i >= 0 -> znth (size xs + i) (xs ++ ys) x = znth i ys x.
-Proof.
-  assert (forall n (xs ys : list instr) i x, i >= 0 -> n = length xs ->
-                                             znth (Z.of_nat n + i) (xs ++ ys) x = znth i ys x);
-    [idtac | scrush].
-  induction n.
-  - scrush.
-  - assert (HH: Z.of_nat (S n) = Z.of_nat n + 1) by
-        Reconstr.htrivial Reconstr.Empty
-		          (@Coq.ZArith.Znat.Nat2Z.inj_succ)
-		          (@Coq.ZArith.BinIntDef.Z.succ).
-    rewrite HH; clear HH.
-    intros xs ys i x H1 H2.
-    assert (0 <= Z.of_nat n + i) by omega.
-    assert (HH: Z.of_nat n + 1 + i = (Z.of_nat n + i) + 1) by omega.
-    rewrite HH; clear HH.
-    destruct xs; [ scrush | simpl ].
-    rewrite lem_n_succ_znth by scrush.
-    scrush.
 Qed.
 
 Lemma lem_exec1_appendL :
@@ -221,16 +220,16 @@ Proof.
   rewrite lem_znth_app by scrush.
   split; [ scrush | split ].
   - Reconstr.htrivial Reconstr.AllHyps
-		      (@lem_iexec_shift)
-		      Reconstr.Empty.
+                      (@lem_iexec_shift)
+                      Reconstr.Empty.
   - split.
     + Reconstr.hobvious Reconstr.AllHyps
-		        (@Coq.ZArith.Zorder.Zle_0_nat, @Coq.ZArith.BinInt.Z.nle_gt,
+                        (@Coq.ZArith.Zorder.Zle_0_nat, @Coq.ZArith.BinInt.Z.nle_gt,
                          @Coq.ZArith.BinInt.Z.add_neg_cases)
-		        (@size, @Coq.ZArith.BinInt.Z.ge, @Coq.ZArith.BinInt.Z.lt).
+                        (@size, @Coq.ZArith.BinInt.Z.ge, @Coq.ZArith.BinInt.Z.lt).
     + Reconstr.hobvious Reconstr.AllHyps
-		        (@lem_size_app, @Coq.ZArith.BinInt.Z.add_lt_mono_l)
-		        (@size).
+                        (@lem_size_app, @Coq.ZArith.BinInt.Z.add_lt_mono_l)
+                        (@size).
 Qed.
 
 Lemma lem_exec_appendL :
@@ -266,4 +265,167 @@ Proof.
   pose lem_exec_appendL; scrush.
 Qed.
 
-(* To be finished... *)
+Lemma lem_exec_appendL_if :
+  forall i i' j P P' s s' stk stk',
+    size P' <= i -> exec P (i - size P',s,stk) (j,s',stk') -> i' = size P' + j ->
+    exec (P' ++ P) (i,s,stk) (i',s',stk').
+Proof.
+  intros.
+  pose (k := i - size P').
+  assert (HH: i = size P' + k) by
+      Reconstr.htrivial Reconstr.Empty
+                        (@Coq.ZArith.BinInt.Zplus_minus)
+                        (@k).
+  rewrite HH; clear HH.
+  pose lem_exec_appendL; scrush.
+Qed.
+
+Lemma lem_exec_append_trans :
+  forall i' i'' j'' P P' s s' s'' stk stk' stk'',
+    exec P (0,s,stk) (i',s',stk') -> size P <= i' ->
+    exec P' (i' - size P,s',stk') (i'',s'',stk'') ->
+    j'' = size P + i'' ->
+    exec (P ++ P') (0,s,stk) (j'',s'',stk'').
+Proof.
+  intros.
+  assert (exec (P ++ P') (i',s',stk') (j'',s'',stk'')) by
+      (apply lem_exec_appendL_if with (j := i''); sauto).
+  assert (exec (P ++ P') (0,s,stk) (i',s',stk')) by
+      (apply lem_exec_appendR; sauto).
+  pose @lem_star_trans; scrush.
+Qed.
+
+Ltac escrush := unfold exec; pose @star_step; pose @star_refl; scrush.
+
+Ltac exec_tac :=
+  match goal with
+  | [ |- exec ?A (?i, ?s, ?stk) ?B ] =>
+    assert (exec1 A (i, s, stk) B) by
+        (unfold exec1; exists i; exists s; exists stk; sauto);
+    escrush
+  end.
+
+Ltac exec_append_tac :=
+  intros; assert (H_exec_append_tac: forall l, size l - size l = 0) by (intro; omega);
+  match goal with
+  | [ |- exec (?l1 ++ ?l2) (0,?s,?stk) (size(?l1 ++ ?l2), ?s, ?a :: ?b :: ?stk) ] =>
+    rewrite lem_size_app;
+    apply lem_exec_append_trans with
+    (i' := size(l1)) (i'' := size(l2)) (s' := s) (stk' := b :: stk);
+    scrush
+  | [ H1 : exec ?l1 (0,?s,?stk) (size(?l1), ?s, ?stk1),
+      H2 : exec ?l2 (0,?s,?stk1) (size(?l2) + ?i, ?s, ?stk2)
+      |- exec (?l1 ++ ?l2) (0,?s,?stk) (size(?l1 ++ ?l2) + ?i, ?s, ?stk2) ] =>
+    rewrite lem_size_app;
+    apply lem_exec_append_trans with
+    (i' := size(l1)) (i'' := size(l2) + i) (s' := s) (stk' := stk1);
+    try omega; ycrush; scrush
+  end;
+  clear H_exec_append_tac.
+
+(* Compilation *)
+
+Fixpoint acomp (a : aexpr) : list instr :=
+  match a with
+  | Anum n => LOADI n :: nil
+  | Avar x => LOAD x :: nil
+  | Aplus a1 a2 => acomp a1 ++ acomp a2 ++ (ADD :: nil)
+  end.
+
+Lemma lem_acomp_correct :
+  forall a s stk, exec (acomp a) (0,s,stk) (size(acomp a),s, aval s a :: stk).
+Proof.
+  induction a; sauto.
+  - exec_tac.
+  - exec_tac.
+  - assert (exec (acomp a1 ++ acomp a2) (0,s,stk)
+                 (size(acomp a1 ++ acomp a2),s,aval s a2 :: aval s a1 :: stk)) by exec_append_tac.
+    assert (exec (ADD :: nil) (0,s,aval s a2 :: aval s a1 :: stk) (1,s,(aval s a1 + aval s a2) :: stk)) by
+        exec_tac.
+    assert (forall l, size l - size l = 0) by (intro; omega);
+    assert (HH: exec ((acomp a1 ++ acomp a2) ++ ADD :: nil) (0, s, stk)
+                     (size ((acomp a1 ++ acomp a2) ++ ADD :: nil), s, aval s a1 + aval s a2 :: stk)) by
+        (apply lem_exec_append_trans with
+         (i' := size(acomp a1 ++ acomp a2)) (s' := s) (stk' := aval s a2 :: aval s a1 :: stk) (i'' := 1);
+         solve [ sauto | ycrush | rewrite lem_size_app; scrush ]).
+    clear -HH; scrush.
+Qed.
+
+Lemma lem_acomp_append :
+   forall a1 a2 s stk, exec (acomp a1 ++ acomp a2) (0, s, stk)
+                            (size (acomp a1 ++ acomp a2), s, aval s a2 :: aval s a1 :: stk).
+Proof.
+  pose lem_acomp_correct; exec_append_tac.
+Qed.
+
+Fixpoint bcomp (b : bexpr) (f : bool) (n : Z) : list instr :=
+  match b with
+  | Bval v => if eqb v f then JMP n :: nil else nil
+  | Bnot b' => bcomp b' (negb f) n
+  | Band b1 b2 =>
+    let cb2 := bcomp b2 f n in
+    let m := if f then size cb2 else size cb2 + n in
+    let cb1 := bcomp b1 false m in
+    cb1 ++ cb2
+  | Bless a1 a2 =>
+    acomp a1 ++ acomp a2 ++ (if f then JMPLESS n :: nil else JMPGE n :: nil)
+  end.
+
+Lemma lem_bcomp_correct :
+  forall b f n s stk, 0 <= n ->
+                      exec (bcomp b f n) (0,s,stk)
+                           (size(bcomp b f n) + (if eqb f (bval s b) then n else 0),s,stk).
+Proof.
+  induction b; simpl; intros f n s stk H.
+  - sauto; try exec_tac;
+      Reconstr.hsimple Reconstr.AllHyps
+                       (@Coq.Bool.Bool.eqb_false_iff, @Coq.Bool.Bool.eqb_prop)
+                       Reconstr.Empty.
+  - assert (HH: (if eqb f (negb (bval s b)) then n else 0) =
+                (if eqb (negb f) (bval s b) then n else 0)) by
+        Reconstr.hsimple Reconstr.Empty
+                         (@Coq.Bool.Bool.eqb_negb2, @Coq.Bool.Bool.negb_false_iff,
+                          @Coq.Bool.Bool.negb_true_iff, @Coq.Bool.Bool.no_fixpoint_negb,
+                          @Coq.Bool.Bool.negb_involutive, @Coq.Bool.Bool.diff_true_false,
+                          @Coq.Bool.Bool.eqb_false_iff, @Coq.Bool.Bool.eqb_prop)
+                         (@Coq.Bool.Bool.eqb, @Coq.Init.Datatypes.negb).
+    rewrite HH; clear HH.
+    scrush.
+  - pose (m := if f then size (bcomp b2 f n) else size (bcomp b2 f n) + n); fold m.
+    assert (H0: 0 <= m) by
+        (unfold m; clear -H; sauto; unfold size; omega).
+    destruct (bval s b1) eqn:H1; simpl.
+    + apply lem_exec_append_trans with
+      (i' := size (bcomp b1 false m))
+        (s' := s) (stk' := stk)
+        (i'' := size (bcomp b2 f n) + (if eqb f (bval s b2) then n else 0)).
+      * generalize (IHb1 false m s stk); scrush.
+      * auto with zarith.
+      * assert (HH: size (bcomp b1 false m) - size (bcomp b1 false m) = 0) by omega.
+        rewrite HH; clear HH.
+        auto.
+      * rewrite lem_size_app; auto with zarith.
+    + rewrite lem_size_app.
+      assert (HH: size (bcomp b2 f n) + (if eqb f false then n else 0) = m) by
+          (unfold m; destruct f; simpl; omega).
+      rewrite <- ZArith.BinInt.Z.add_assoc; rewrite HH; clear HH.
+      apply lem_exec_appendR.
+      assert (HH: size (bcomp b1 false m) + m =
+                  size (bcomp b1 false m) + if eqb false (bval s b1) then m else 0) by scrush.
+      rewrite HH; clear HH.
+      auto.
+  - assert (HH: aval s a >=? aval s a0 = negb (aval s a <? aval s a0)) by
+        Reconstr.htrivial Reconstr.Empty
+                          (@Coq.ZArith.BinInt.Z.geb_leb, @Coq.Bool.Bool.negb_true_iff,
+                           @Coq.ZArith.BinInt.Z.leb_antisym)
+                          Reconstr.Empty.
+    assert (exec (if f then JMPLESS n :: nil else JMPGE n :: nil) (0, s, aval s a0 :: aval s a :: stk)
+                 (size (if f then JMPLESS n :: nil else JMPGE n :: nil) +
+                  (if eqb f (aval s a <? aval s a0) then n else 0), s, stk)) by
+        (sauto; exec_tac).
+    clear HH.
+    assert (HH: forall (l1 l2 l3 : list instr), l1 ++ l2 ++ l3 = (l1 ++ l2) ++ l3) by scrush.
+    repeat rewrite HH; clear HH.
+    pose proof (lem_acomp_append a a0 s stk).
+    exec_append_tac.
+Qed.
